More annotations are needed to keep bytes from turning into seq uint8

contrib/Platform/fst/Platform.Bytes.fst
@@ -40,6 +40,10 @@ type byte = uint8
 type cbytes = string
 opaque type bytes = Seq.seq byte
 
+val seq_of_bytes: b:bytes -> GTot (Seq.seq byte)
+let seq_of_bytes b = b
+
+val op_At_Bar: bytes -> bytes -> Tot bytes
 let op_At_Bar (b1:bytes) (b2:bytes) = Seq.append b1 b2
 
 (*@ function val B : (bytes -> byte array) @*)
@@ -94,6 +98,7 @@ assume val xor: l:nat -> lbytes l -> lbytes l -> Tot (lbytes l)
 
 //val split: b:bytes -> n:nat{n <= Seq.length b} -> 
 //  Tot (x:(bytes * bytes) {Seq.length (fst (x))= n /\ Seq.length (snd (x)) == (Seq.length b) - n }) //(lbytes n * lbytes (length b - n))
+val split: bytes -> nat -> Tot (bytes * bytes)
 let split b (n:nat { n <= Seq.length b}) = SeqProperties.split b n
 
 val lemma_split : s:bytes -> i:nat{(0 <= i /\ i <= length s)} -> Lemma
